feat: Array.zipWithAll (#6191)
This PR adds `Array.zipWithAll`, and the basic lemmas relating it to
`List.zipWithAll`.

src/Init/Data/Array/Basic.lean
@@ -13,6 +13,7 @@ import Init.Data.ToString.Basic
 import Init.GetElem
 import Init.Data.List.ToArray
 import Init.Data.Array.Set
+
 universe u v w
 
 /-! ### Array literal syntax -/
@@ -883,12 +884,12 @@ def isPrefixOf [BEq α] (as bs : Array α) : Bool :=
     false
 
 @[semireducible, specialize] -- This is otherwise irreducible because it uses well-founded recursion.
-def zipWithAux (f : α → β → γ) (as : Array α) (bs : Array β) (i : Nat) (cs : Array γ) : Array γ :=
+def zipWithAux (as : Array α) (bs : Array β) (f : α → β → γ) (i : Nat) (cs : Array γ) : Array γ :=
   if h : i < as.size then
     let a := as[i]
     if h : i < bs.size then
       let b := bs[i]
-      zipWithAux f as bs (i+1) <| cs.push <| f a b
+      zipWithAux as bs f (i+1) <| cs.push <| f a b
     else
       cs
   else
@@ -896,10 +897,22 @@ def zipWithAux (f : α → β → γ) (as : Array α) (bs : Array β) (i : Nat) 
 decreasing_by simp_wf; decreasing_trivial_pre_omega
 
 @[inline] def zipWith (as : Array α) (bs : Array β) (f : α → β → γ) : Array γ :=
-  zipWithAux f as bs 0 #[]
+  zipWithAux as bs f 0 #[]
 
 def zip (as : Array α) (bs : Array β) : Array (α × β) :=
   zipWith as bs Prod.mk
+
+def zipWithAll (as : Array α) (bs : Array β) (f : Option α → Option β → γ) : Array γ :=
+  go as bs 0 #[]
+where go (as : Array α) (bs : Array β) (i : Nat) (cs : Array γ) :=
+  if i < max as.size bs.size then
+    let a := as[i]?
+    let b := bs[i]?
+    go as bs (i+1) (cs.push (f a b))
+  else
+    cs
+  termination_by max as.size bs.size - i
+  decreasing_by simp_wf; decreasing_trivial_pre_omega
 
 def unzip (as : Array (α × β)) : Array α × Array β :=
   as.foldl (init := (#[], #[])) fun (as, bs) (a, b) => (as.push a, bs.push b)
